Added "uniqueness" predicate
seqConjunction and seqConjunction are set operations on sequences, and the assumption here is that the arguments to those functions, although defined as sequences, are, for all practical concerns, actually sets, which means their members are unique.

Util.dfy
@@ -36,6 +36,8 @@ ensures forall c :: c in res ==> '\u0030' <= c <= '\u0039'
 
 /* res := X*Y */
 function method {:verify true} seqConjunction<T(==)>(X: seq<T>, Y: seq<T>) : (res: seq<T>)
+requires uniqueness(X)
+requires uniqueness(Y)
 ensures forall i :: i in res ==> i in X && i in Y
 ensures forall i :: i !in res ==> i !in X || i !in Y
 {
@@ -44,8 +46,12 @@ ensures forall i :: i !in res ==> i !in X || i !in Y
 	else seqConjunction(X[1..], Y)
 }
 
+
 /* res := X-Y */
 function method {:verify true} seqSubtraction<T(==)>(X: seq<T>, Y: seq<T>) : (res: seq<T>)
+requires uniqueness(X)
+requires uniqueness(Y)
+decreases X
 ensures forall i :: i in res ==> i in X && i !in Y
 ensures forall i :: i !in res ==> i !in X || i in Y
 {
@@ -53,4 +59,9 @@ ensures forall i :: i !in res ==> i !in X || i in Y
 	else if Y == [] then X
 	else if X[0] in Y then seqSubtraction(X[1..], Y)
 	else [X[0]]+seqSubtraction(X[1..], Y)
+}
+
+predicate uniqueness<T(==)>(X: seq<T>)
+{
+	(forall i,j :: i in X && j in X && i != j) ==> true
 }
